proof/invariant-abstract/X64/Machine_AI.thy
@@ -1,4 +1,5 @@
 (*
+ * Copyright 2025, Proofcraft Pty Ltd
  * Copyright 2014, General Dynamics C4 Systems
  *
  * SPDX-License-Identifier: GPL-2.0-only
@@ -12,6 +13,7 @@ theory Machine_AI
 imports Bits_AI
 begin
 
+text \<open>Crunch setup\<close>
 
 definition
   "no_irq f \<equiv> \<forall>P. \<lbrace>\<lambda>s. P (irq_masks s)\<rbrace> f \<lbrace>\<lambda>_ s. P (irq_masks s)\<rbrace>"
@@ -69,94 +71,56 @@ crunch_ignore (no_irq) (add:
 
 context Arch begin arch_global_naming
 
+text \<open>Deterministic\<close>
+
 lemma det_getRegister: "det (getRegister x)"
   by (simp add: getRegister_def)
 
 lemma det_setRegister: "det (setRegister x w)"
   by (simp add: setRegister_def det_def modify_def get_def put_def bind_def)
 
-
 lemma det_getRestartPC: "det getRestartPC"
   by (simp add: getRestartPC_def det_getRegister)
-
 
 lemma det_setNextPC: "det (setNextPC p)"
   by (simp add: setNextPC_def det_setRegister)
 
-(* FIXME empty_fail: make all empty_fail [intro!, wp], and non-conditional ones [simp] *)
-lemma ef_loadWord: "empty_fail (loadWord x)"
-  by (fastforce simp: loadWord_def)
+text \<open>Failure on empty result\<close>
 
+crunch loadWord, storeWord, machine_op_lift
+  for (empty_fail) empty_fail[intro!, wp, simp]
+  (ignore: Nondet_Monad.bind mapM_x simp: machine_op_lift_def empty_fail_cond)
 
-lemma ef_storeWord: "empty_fail (storeWord x y)"
-  by (fastforce simp: storeWord_def)
+lemmas ef_machine_op_lift = machine_op_lift_empty_fail \<comment> \<open>required for generic interface\<close>
 
+text \<open>Does not affect state\<close>
 
-lemma no_fail_getRestartPC: "no_fail \<top> getRestartPC"
+definition "irq_state_independent P \<equiv> \<forall>f s. P s \<longrightarrow> P (irq_state_update f s)"
+
+lemma getActiveIRQ_inv[wp]:
+  "\<lbrakk>irq_state_independent P\<rbrakk> \<Longrightarrow> getActiveIRQ in_kernel \<lbrace>P\<rbrace>"
+  apply (simp add: getActiveIRQ_def)
+  apply wp
+  apply (simp add: irq_state_independent_def)
+  done
+
+lemma loadWord_inv[wp]: "loadWord x \<lbrace>P\<rbrace>"
+  by (wpsimp simp: loadWord_def)
+
+lemma getRestartPC_inv: "getRestartPC \<lbrace>P\<rbrace>"
   by (simp add: getRestartPC_def getRegister_def)
 
+text \<open>Does not set failure flag\<close>
 
-lemma no_fail_loadWord [wp]: "no_fail (\<lambda>_. is_aligned p 3) (loadWord p)"
-  apply (simp add: loadWord_def is_aligned_mask [symmetric])
-  apply (rule no_fail_pre)
-   apply wp
-  apply simp
-  done
-
+lemma no_fail_loadWord[wp]: "no_fail (\<lambda>_. is_aligned p 3) (loadWord p)"
+  by (wpsimp simp: loadWord_def is_aligned_mask [symmetric])
 
 lemma no_fail_storeWord: "no_fail (\<lambda>_. is_aligned p 3) (storeWord p w)"
-  apply (simp add: storeWord_def is_aligned_mask [symmetric])
-  apply (rule no_fail_pre)
-   apply (wp)
-  apply simp
-  done
-
+  by (wpsimp simp: storeWord_def is_aligned_mask [symmetric])
 
 lemma no_fail_machine_op_lift [simp]:
   "no_fail \<top> (machine_op_lift f)"
   by (simp add: machine_op_lift_def)
-
-
-lemma ef_machine_op_lift [simp]:
-  "empty_fail (machine_op_lift f)"
-  by (simp add: machine_op_lift_def)
-
-
-
-lemma no_fail_setNextPC: "no_fail \<top> (setNextPC pc)"
-  by (simp add: setNextPC_def setRegister_def)
-
-
-lemma no_fail_initL2Cache: "no_fail \<top> initL2Cache"
-  by (simp add: initL2Cache_def)
-
-lemma no_fail_resetTimer[wp]: "no_fail \<top> resetTimer"
-  by (simp add: resetTimer_def)
-
-
-lemma loadWord_inv: "\<lbrace>P\<rbrace> loadWord x \<lbrace>\<lambda>x. P\<rbrace>"
-  apply (simp add: loadWord_def)
-  apply wp
-  apply simp
-  done
-
-
-lemma getRestartPC_inv: "\<lbrace>P\<rbrace> getRestartPC \<lbrace>\<lambda>rv. P\<rbrace>"
-  by (simp add: getRestartPC_def getRegister_def)
-
-
-
-lemma no_fail_clearMemory[simp, wp]:
-  "no_fail (\<lambda>_. is_aligned p 3) (clearMemory p b)"
-  apply (simp add: clearMemory_def mapM_x_mapM)
-  apply (rule no_fail_pre)
-   apply (wp no_fail_mapM' no_fail_storeWord )
-  apply (clarsimp simp: upto_enum_step_def)
-  apply (erule aligned_add_aligned)
-   apply (simp add: word_size_def)
-   apply (rule is_aligned_mult_triv2 [where n = 3, simplified])
-  apply simp
-  done
 
 lemma no_fail_freeMemory[simp, wp]:
   "no_fail (\<lambda>_. is_aligned p 3) (freeMemory p b)"
@@ -170,7 +134,6 @@ lemma no_fail_freeMemory[simp, wp]:
   apply simp
   done
 
-
 lemma no_fail_getActiveIRQ[wp]:
   "no_fail \<top> (getActiveIRQ in_kernel)"
   apply (simp add: getActiveIRQ_def)
@@ -179,23 +142,12 @@ lemma no_fail_getActiveIRQ[wp]:
   apply simp
   done
 
-definition "irq_state_independent P \<equiv> \<forall>f s. P s \<longrightarrow> P (irq_state_update f s)"
+text \<open>Does not affect IRQ masks - low-level properties of @{term no_irq}\<close>
 
-lemma getActiveIRQ_inv [wp]:
-  "\<lbrakk>irq_state_independent P\<rbrakk> \<Longrightarrow> \<lbrace>P\<rbrace> getActiveIRQ in_kernel \<lbrace>\<lambda>rv. P\<rbrace>"
-  apply (simp add: getActiveIRQ_def)
-  apply wp
-  apply (simp add: irq_state_independent_def)
-  done
-
-lemma no_fail_ackInterrupt[wp]: "no_fail \<top> (ackInterrupt irq)"
-  by (simp add: ackInterrupt_def)
-
-
-lemma no_fail_maskInterrupt[wp]: "no_fail \<top> (maskInterrupt irq bool)"
-  by (simp add: maskInterrupt_def)
-
-
+lemma no_irq_bind[wp]:
+  "\<lbrakk> no_irq f; \<And>rv. no_irq (g rv) \<rbrakk> \<Longrightarrow> no_irq (f >>= g)"
+  unfolding no_irq_def
+  by (wpsimp, blast+)
 
 lemma no_irq_use:
   "\<lbrakk> no_irq f; (rv,s') \<in> fst (f s) \<rbrakk> \<Longrightarrow> irq_masks s' = irq_masks s"
@@ -204,12 +156,9 @@ lemma no_irq_use:
   apply fastforce
   done
 
-lemma no_irq_machine_rest_lift:
+lemma no_irq_machine_rest_lift[simp, wp]:
   "no_irq (machine_rest_lift f)"
-  apply (clarsimp simp: no_irq_def machine_rest_lift_def split_def)
-  apply wp
-  apply simp
-  done
+  by (wpsimp simp: no_irq_def machine_rest_lift_def split_def)
 
 crunch machine_op_lift
   for (no_irq) no_irq[wp, simp]
@@ -218,90 +167,40 @@ lemma no_irq:
   "no_irq f \<Longrightarrow> \<lbrace>\<lambda>s. P (irq_masks s)\<rbrace> f \<lbrace>\<lambda>_ s. P (irq_masks s)\<rbrace>"
   by (simp add: no_irq_def)
 
-lemma no_irq_invalidateTLB: "no_irq  invalidateTLB"
-  by (simp add: invalidateTLB_def)
+lemma no_irq_return[simp, wp]:
+  "no_irq (return v)"
+  unfolding no_irq_def
+  by simp
 
-lemma no_irq_initL2Cache: "no_irq  initL2Cache"
-  by (simp add: initL2Cache_def)
+lemma no_irq_get[simp, wp]:
+  "no_irq get"
+  by (wpsimp simp: no_irq_def)
 
-lemma no_irq_gets [simp]:
+lemma no_irq_gets[simp, wp]:
   "no_irq (gets f)"
   by (simp add: no_irq_def)
 
-
-lemma no_irq_resetTimer: "no_irq resetTimer"
-  by (simp add: resetTimer_def)
-
-
-lemma no_irq_debugPrint: "no_irq (debugPrint $ xs)"
-  by (simp add: no_irq_def)
-
-context notes no_irq[wp] begin
-
-lemma no_irq_ackInterrupt: "no_irq (ackInterrupt irq)"
-  by (wp | clarsimp simp: no_irq_def ackInterrupt_def)+
-
-lemma no_irq_writeCR3: "no_irq (writeCR3 vs asid)"
-  by (wp | clarsimp simp: no_irq_def writeCR3_def)+
-
-lemma no_irq_loadWord: "no_irq (loadWord x)"
-  apply (clarsimp simp: no_irq_def)
-  apply (rule loadWord_inv)
-  done
-
-
-lemma no_irq_getActiveIRQ: "no_irq (getActiveIRQ in_kernel)"
-  apply (clarsimp simp: no_irq_def)
-  apply (rule getActiveIRQ_inv)
-  apply (simp add: irq_state_independent_def)
-  done
-
-
 lemma no_irq_mapM:
   "(\<And>x. x \<in> set xs \<Longrightarrow> no_irq (f x)) \<Longrightarrow> no_irq (mapM f xs)"
-  apply (subst no_irq_def)
-  apply clarify
-  apply (rule mapM_wp)
-   prefer 2
-   apply (rule order_refl)
-  apply (wp; simp)
+  apply (simp (no_asm) add: no_irq_def)
+  apply (clarsimp intro!: mapM_wp[OF _ order_refl])
+  apply (wpsimp wp: no_irq)
   done
-
 
 lemma no_irq_mapM_x:
   "(\<And>x. x \<in> set xs \<Longrightarrow> no_irq (f x)) \<Longrightarrow> no_irq (mapM_x f xs)"
-  apply (subst no_irq_def)
-  apply clarify
-  apply (rule mapM_x_wp)
-   prefer 2
-   apply (rule order_refl)
-  apply (wp; simp)
+  apply (simp (no_asm) add: no_irq_def)
+  apply (clarsimp intro!: mapM_x_wp[OF _ order_refl])
+  apply (wpsimp wp: no_irq)
   done
-
 
 lemma no_irq_swp:
   "no_irq (f y x) \<Longrightarrow> no_irq (swp f x y)"
   by (simp add: swp_def)
 
-
-lemma no_irq_seq [wp]:
-  "\<lbrakk> no_irq f; \<And>x. no_irq (g x) \<rbrakk> \<Longrightarrow> no_irq (f >>= g)"
-  apply (subst no_irq_def)
-  apply clarsimp
-  apply (rule bind_wp)
-  apply (wp|simp)+
-  done
-
-lemma no_irq_return [simp, wp]: "no_irq (return v)"
-  unfolding no_irq_def return_def
-  by (rule allI, simp add: valid_def)
-
-
 lemma no_irq_fail [simp, wp]: "no_irq fail"
   unfolding no_irq_def fail_def
   by (rule allI, simp add: valid_def)
-
-
 
 lemma no_irq_assert [simp, wp]: "no_irq (assert P)"
   unfolding assert_def by simp
@@ -313,82 +212,175 @@ lemma no_irq_modify:
   apply (clarsimp simp: in_monad)
   done
 
-lemma no_irq_invalidateTLBEntry: "no_irq (invalidateTLBEntry a)"
-  by (clarsimp simp: invalidateTLBEntry_def)
-
-lemma no_irq_storeWord: "no_irq (storeWord w p)"
-  apply (simp add: storeWord_def)
-  apply (wp no_irq_modify)
-  apply simp
-  done
-
-lemma no_irq_when:
+lemma no_irq_when[simp, wp]:
   "\<lbrakk>P \<Longrightarrow> no_irq f\<rbrakk> \<Longrightarrow> no_irq (when P f)"
   by (simp add: when_def)
 
-lemma no_irq_clearMemory: "no_irq (clearMemory a b)"
-  apply (simp add: clearMemory_def)
-  apply (wp no_irq_mapM_x no_irq_storeWord)
+text \<open>Architecture-specific @{term no_irq} preservations\<close>
+
+lemma no_irq_loadWord: "no_irq (loadWord x)"
+  by (wpsimp simp: no_irq_def wp: loadWord_inv)
+
+lemma no_irq_getActiveIRQ: "no_irq (getActiveIRQ in_kernel)"
+  by (wpsimp simp: no_irq_def irq_state_independent_def wp: getActiveIRQ_inv)
+
+lemma no_irq_storeWord: "no_irq (storeWord w p)"
+  by (wpsimp simp: storeWord_def wp: no_irq_modify)
+
+crunch ackInterrupt
+  for (no_irq) no_irq[intro!, wp, simp]
+
+text \<open>Wide-angle crunch proofs over architecture-specific machine operations for
+  @{term no_fail}, @{term empty_fail} and @{term no_irq}}}\<close>
+
+(* Most of the basic machine ops in MachineOps.thy use abstract _impl constants which should never
+   be expanded.
+   Note: this was generated by running the following, and should likely be updated the same way:
+   grep -o "\w\+_impl" MachineOps.thy|sort|uniq|sed "s/^/    /"
+   *)
+crunch_ignore (valid, empty_fail, no_fail)
+  (add:
+    configureTimer_impl
+    disableFpu_impl
+    enableFpu_impl
+    getDeviceRegions_impl
+    getKernelDevices_impl
+    in16_impl
+    in32_impl
+    in8_impl
+    initL2Cache_impl
+    initTimer_impl
+    invalidateASID_impl
+    invalidateLocalPageStructureCacheASID_impl
+    invalidateTLBEntry_impl
+    invalidateTLB_impl
+    invalidateTranslationSingleASID_impl
+    ioapicMapPinToVector_impl
+    mfence_impl
+    out16_impl
+    out32_impl
+    out8_impl
+    resetTimer_impl
+    writeCR3_impl
+    writeFpuState_impl
+    )
+
+(* Crunches for machine ops without concrete implementations (using _impl or _val).
+   List obtained using:
+   grep -oE "(\w+_impl)|(get\w+)" MachineOps.thy|sort|uniq|sed "s/_impl//;s/$/,/;s/^/  /"
+   with the following manual interventions:
+   - remove false positives: get_def, gets, gets_def, getFPUState, getRegister, getRestartPC,
+                             getDeviceRegions_val, getFaultAddress_val, getKernelDevices_val
+   - add read_cntpct and readFpuState
+   - remove final comma
+   - getActiveIRQ does not preserve no_irq *)
+crunch
+  configureTimer,
+  disableFpu,
+  enableFpu,
+  getDeviceRegions,
+  getDeviceRegions,
+  getFaultAddress,
+  getKernelDevices,
+  getKernelDevices,
+  getMemoryRegions,
+  in16,
+  in32,
+  in8,
+  initL2Cache,
+  initTimer,
+  invalidateASID,
+  invalidateLocalPageStructureCacheASID,
+  invalidateTLBEntry,
+  invalidateTLB,
+  invalidateTranslationSingleASID,
+  ioapicMapPinToVector,
+  mfence,
+  out16,
+  out32,
+  out8,
+  resetTimer,
+  writeCR3,
+  writeFpuState,
+  readFpuState
+  for (no_fail) no_fail[intro!, wp, simp]
+  and (empty_fail) empty_fail[intro!, wp, simp]
+  and (no_irq) no_irq[intro!, wp, simp]
+  and device_state_inv[wp]: "\<lambda>ms. P (device_state ms)"
+  and irq_masks[wp]: "\<lambda>s. P (irq_masks s)"
+  and underlying_memory_inv[wp]: "\<lambda>s. P (underlying_memory s)"
+  (wp: no_irq_bind no_irq_modify ef_machine_rest_lift no_fail_machine_state_rest_T)
+
+crunch getFPUState, getRegister, getRestartPC, setNextPC, ackInterrupt, maskInterrupt, hwASIDInvalidate
+  for (no_fail) no_fail[intro!, wp, simp]
+  and (empty_fail) empty_fail[intro!, wp, simp]
+
+crunch ackInterrupt, maskInterrupt
+  for device_state_inv[wp]: "\<lambda>ms. P (device_state ms)"
+  and underlying_memory_inv[wp]: "\<lambda>s. P (underlying_memory s)"
+
+crunch ackInterrupt
+  for irq_masks[wp]: "\<lambda>s. P (irq_masks s)"
+
+text \<open>Lifting rules\<close>
+
+lemma dmo_machine_state_lift:
+  "\<lbrace>P\<rbrace> f \<lbrace>Q\<rbrace> \<Longrightarrow> \<lbrace>\<lambda>s. P (machine_state s)\<rbrace> do_machine_op f \<lbrace>\<lambda>rv s. Q rv (machine_state s)\<rbrace>"
+  unfolding do_machine_op_def by wpsimp (erule use_valid; assumption)
+
+crunch do_machine_op
+  for user_frame[wp]: "\<lambda>s. P (in_user_frame p s)"
+
+lemma dmo_valid_machine_state[wp]:
+  assumes "\<And>P. f \<lbrace>\<lambda>s. P (underlying_memory s)\<rbrace>"
+  shows "do_machine_op f \<lbrace>valid_machine_state\<rbrace>"
+  unfolding valid_machine_state_def
+  by (wpsimp wp: hoare_vcg_all_lift hoare_vcg_disj_lift dmo_machine_state_lift assms)
+
+lemma dmo_valid_irq_states[wp]:
+  "(\<And>P. f \<lbrace>\<lambda>s. P (irq_masks s)\<rbrace>) \<Longrightarrow> do_machine_op f \<lbrace>valid_irq_states\<rbrace>"
+  unfolding valid_irq_states_def do_machine_op_def
+  by (wpsimp, erule use_valid; assumption)
+
+text \<open>Ops that require machine-ops rules derived above\<close>
+
+\<comment> \<open>These can't be placed into the sections above, as they require the derivation of the machine op
+   properties, and those in turn rely on items in specific sections above. There are unlikely to be
+   many definitions like this in MachineOps.thy\<close>
+
+crunch clearMemory
+  for (empty_fail) empty_fail[intro!, wp, simp]
+
+lemma no_fail_clearMemory[unfolded word_size_bits_def, simp, wp]:
+  "no_fail (\<lambda>_. is_aligned p word_size_bits) (clearMemory p b)"
+  apply (simp add: clearMemory_def word_size_bits_def mapM_x_mapM)
+  apply (rule no_fail_pre)
+   apply (wp no_fail_mapM' no_fail_storeWord )
+  apply (clarsimp simp: upto_enum_step_def)
+  apply (erule aligned_add_aligned)
+   apply (simp add: word_size_def)
+   apply (rule is_aligned_mult_triv2 [where n = 3, simplified])
+  apply simp
   done
 
-lemma no_irq_in8: "no_irq (in8 irq)"
-  by (wp | clarsimp simp: in8_def)+
+lemma no_irq_clearMemory: "no_irq (clearMemory a b)"
+  by (wpsimp simp: clearMemory_def no_irq_mapM_x no_irq_storeWord)
 
-lemma no_irq_in16: "no_irq (in16 irq)"
-  by (wp | clarsimp simp: in16_def)+
-
-lemma no_irq_in32: "no_irq (in32 irq)"
-  by (wp | clarsimp simp: in32_def)+
-
-lemma no_irq_out8: "no_irq (out8 irq b)"
-  by (wp | clarsimp simp: out8_def)+
-
-lemma no_irq_out16: "no_irq (out16 irq b)"
-  by (wp | clarsimp simp: out16_def)+
-
-lemma no_irq_out32: "no_irq (out32 irq b)"
-  by (wp | clarsimp simp: out32_def)+
-
-lemma no_irq_invalidateLocalPageStructureCacheASID:
-  "no_irq (invalidateLocalPageStructureCacheASID vspace asid)"
-  by (wpsimp simp: invalidateLocalPageStructureCacheASID_def)
-
-lemmas invalidateLocalPageStructureCacheASID_irq_masks =
-  no_irq[OF no_irq_invalidateLocalPageStructureCacheASID]
-
-lemma no_irq_nativeThreadUsingFPU: "no_irq (nativeThreadUsingFPU thread)"
-  by (wp | clarsimp simp: nativeThreadUsingFPU_def)+
-
-lemma no_irq_switchFpuOwner: "no_irq (switchFpuOwner thread cpu)"
-  by (wp | clarsimp simp: switchFpuOwner_def)+
-
-lemmas nativeThreadUsingFPU_irq_masks = no_irq[OF no_irq_nativeThreadUsingFPU]
-lemmas switchFpuOwner_irq_masks = no_irq[OF no_irq_switchFpuOwner]
+text \<open>Misc WP rules\<close>
 
 lemma getActiveIRQ_le_maxIRQ':
   "\<lbrace>\<lambda>s. \<forall>irq > maxIRQ. irq_masks s irq\<rbrace>
     getActiveIRQ in_kernel
    \<lbrace>\<lambda>rv s. \<forall>x. rv = Some x \<longrightarrow> x \<le> maxIRQ\<rbrace>"
   apply (simp add: getActiveIRQ_def)
-  apply wp
-  apply clarsimp
+  apply wpsimp
   apply (rule ccontr)
   apply (simp add: linorder_not_le)
   done
 
-(* FIXME: follows already from getActiveIRQ_le_maxIRQ *)
-lemma getActiveIRQ_neq_Some0xFF':
-  "\<lbrace>\<top>\<rbrace> getActiveIRQ in_kernel \<lbrace>\<lambda>rv s. rv \<noteq> Some 0x3FF\<rbrace>"
-  apply (simp add: getActiveIRQ_def)
-  apply wpsimp
-  done
-
 lemma getActiveIRQ_neq_non_kernel:
   "\<lbrace>\<top>\<rbrace> getActiveIRQ True \<lbrace>\<lambda>rv s. rv \<notin> Some ` non_kernel_IRQs \<rbrace>"
-  apply (simp add: getActiveIRQ_def)
-  apply wp
-  apply auto
-  done
+  by (wpsimp simp: getActiveIRQ_def)
 
 lemma dmo_getActiveIRQ_non_kernel[wp]:
   "\<lbrace>\<top>\<rbrace> do_machine_op (getActiveIRQ True)
@@ -399,59 +391,10 @@ lemma dmo_getActiveIRQ_non_kernel[wp]:
   apply clarsimp
   done
 
-lemma empty_fail_invalidateTLB: "empty_fail  invalidateTLB"
-  by (simp add: invalidateTLB_def)
+lemma dmo_gets_inv[wp]:
+  "do_machine_op (gets f) \<lbrace>P\<rbrace>"
+  unfolding do_machine_op_def by (wpsimp simp: simpler_gets_def)
 
-lemma empty_fail_initL2Cache: "empty_fail  initL2Cache"
-  by (simp add: initL2Cache_def)
-
-lemma empty_fail_clearMemory [simp, intro!]:
-  "\<And>a b. empty_fail (clearMemory a b)"
-  by (fastforce simp: clearMemory_def mapM_x_mapM ef_storeWord)
-
-lemma getFaultAddress_ef[simp,wp]: "empty_fail getFaultAddress"
-  by (simp add: getFaultAddress_def)
-
-lemma ioapicMapPinToVector_ef[simp,wp]: "empty_fail (ioapicMapPinToVector a b c d e)"
-  by (simp add: ioapicMapPinToVector_def)
-
-lemma invalidateTLBEntry_ef[simp,wp]: "empty_fail (invalidateTLBEntry b)"
-  by (simp add: invalidateTLBEntry_def)
-
-lemma invalidateASID_ef[simp,wp]: "empty_fail (invalidateASID a b)"
-  by (simp add: invalidateASID_def)
-
-lemma invalidateTranslationSingleASID_ef[simp,wp]: "empty_fail (invalidateTranslationSingleASID a b)"
-  by (simp add: invalidateTranslationSingleASID_def)
-
-lemma hwASIDInvalidate_ef[simp,wp]: "empty_fail (hwASIDInvalidate b a)"
-  by (simp add: hwASIDInvalidate_def)
-
-lemma updateIRQState_ef[simp,wp]: "empty_fail (updateIRQState b c)"
-  by (fastforce simp: updateIRQState_def)
-
-lemma writeCR3_ef[simp,wp]: "empty_fail (writeCR3 a b)"
-  by (simp add: writeCR3_def)
-
-lemma in8_ef[simp,wp]: "empty_fail (in8 port)"
-  by (fastforce simp: in8_def)
-
-lemma in16_ef[simp,wp]: "empty_fail (in16 port)"
-  by (fastforce simp: in16_def)
-
-lemma in32_ef[simp,wp]: "empty_fail (in32 port)"
-  by (fastforce simp: in32_def)
-
-lemma out8_ef[simp,wp]: "empty_fail (out8 port dat)"
-  by (simp add: out8_def)
-
-lemma out16_ef[simp,wp]: "empty_fail (out16 port dat)"
-  by (simp add: out16_def)
-
-lemma out32_ef[simp,wp]: "empty_fail (out32 port dat)"
-  by (simp add: out32_def)
-
-end
 end
 
 end
